---
layout: distill
title: A detailed example of Fast Fourier Transform
date: 2024-05-02 9:00:00
description: When learning this topic, I encountered a problem regarding the Twiddle Factor and the butter fly diagram. Here is my explanation with a derivation of 8 point example.  
tags: advanced-transforms algorithms
categories: algorithms

bibliography: 2024-04-27-Hysteresis-voltage.bib

toc:
  -name: Discrete Fourier Transform
  -name: FFT with an 8-point example
  -name: How to read a butterfly diagram
  -name: Connections with butterfly diagram:the elimination of k in twiddle factors
---

## Discrete Fourier Transform

I suppose nobody can get away of Discrete Fourier Transform(DFT) when talking about Fast Fourier Transform(FFT). Let's have a quick look.  

A DFT comes from continuous Fourier Transform:

$$\hat f(\omega) = \mathscr{F}\{f(t)\} = \int_{-\infty}^{+\infty} f(\tau) e^{-i\omega t} dt$$

For a discrete version of FT:

$$\hat f[k] = \frac{1}{N}\sum_{n=0}^{N-1}f[n]e^{-\frac{2\pi i k n }{N}}$$  

Take a detailed look at the $k = 0$ case.  

$$\hat f[k = 0] = \frac{1}{N}(f[0]+f[1]+f[2]+...+f[N-1])$$
$$\hat f[k = 0] =  \frac{1}{N}\sum_{n=0}^{N-1} = \mu = mean$$  

In the background of circuit, this $k = 0$ term is also called a DC-offset.  

$$\hat f[k = 1] = \frac{1}{N}(f[0]+f[1]e^{(\frac{-2\pi i }{N})}+f[2]e^{(\frac{-4\pi i }{N})}+...+f[N-1]e^{(\frac{-2\pi i (N-1)}{N})})$$
$$\hat f[k = 2] = \frac{1}{N}(f[0]+f[1]e^{(\frac{-2*2\pi i }{N})}+f[2]e^{(\frac{-2*4\pi i }{N})}+...+f[N-1]e^{(\frac{-2\pi i 2* (N-1)}{N})})$$  
$$\hat f[k = m] = \frac{1}{N}(f[0]+f[1]e^{(\frac{-m*2\pi i }{N})}+f[2]e^{(\frac{-m*4\pi i }{N})}+...+f[N-1]e^{(\frac{-2\pi i m* (N-1)}{N})})$$  

If we define the *Fundamental Frequency*:  

$$W_N = e^{-\frac{2\pi i }{N}}$$  

Maybe you have noticed that $W_N$ is the last solution to the polinomial equation:  

$$x^N = 1$$  

Anyway, the DFT not becomes:  

$$\hat f[k] = \frac{1}{N}\sum_{n=0}^{N-1}f[n]W_N^{kn}$$  

In a matrix form:  

<div class="row mt-5">
    <div class="col-sm mt-5 mt-md-0">
        {% include figure.liquid loading="eager" path="assets/img/2024-05-02-fft/DFT.png" class="img-fluid rounded z-depth-1" %}
    </div>
</div>

If we calculate DFT in this way, the time complexity is $O(N^2)$.  

## FFT with an 8-point example

One may notice that there are so many $W_N$ in the matrix, we calculate them again and again, and it there any way that we can make life easier and reuse the data we have calculated before. Recursively, we can divide the equation into *odd* and *even* components and they have the same factor and we can re-divide the equation into sub-*odd* and sub-*even* components and so on and so forth. This could result in a beautiful algorithm that can be explained with a butterfly diagram.  Do not panic if you cannot understand what I am saying, I will explain this with an 8-point example.  

<div class="row mt-5">
    <div class="col-sm mt-5 mt-md-0">
        {% include figure.liquid loading="eager" path="assets/img/2024-05-02-fft/8p1.png" class="img-fluid rounded z-depth-1" %}
    </div>
</div>

I delibrately write the equation in a form of even and odd terms.  
<div class="row mt-5">
    <div class="col-sm mt-5 mt-md-0">
        {% include figure.liquid loading="eager" path="assets/img/2024-05-02-fft/8p2.png" class="img-fluid rounded z-depth-1" %}
    </div>
</div>

Now the odd and even term has a same factor.  

The $e^{-\frac{2\pi i k}{8}}$ is called *twiddle factor*.  

$$W_t = W_M^k$$  
You will see that the $M$ will be divided from N by a factor of 2 every time we separate the odd and even terms. **Please note that there is a important $k$ thing in the exponential term**, which actually causes more trouble to understand the FFT. I did not notice that at first and thought I understood FFT. However, when going over the whole materials, I noticed that k thing and realised that I just did not understand FFT.  

We can do the same thing 2 more times:  

<div class="row mt-5">
    <div class="col-sm mt-5 mt-md-0">
        {% include figure.liquid loading="eager" path="assets/img/2024-05-02-fft/8p3.png" class="img-fluid rounded z-depth-1" %}
    </div>
</div>

Notice in the exponential term, we can divide both numerator and denominator by a 2.  

<div class="row mt-5">
    <div class="col-sm mt-5 mt-md-0">
        {% include figure.liquid loading="eager" path="assets/img/2024-05-02-fft/8p4.png" class="img-fluid rounded z-depth-1" %}
    </div>
</div>

Get new twiddle factor out:  
 
<div class="row mt-5">
    <div class="col-sm mt-5 mt-md-0">
        {% include figure.liquid loading="eager" path="assets/img/2024-05-02-fft/8p5.png" class="img-fluid rounded z-depth-1" %}
    </div>
</div>

Divide both numerator and denominator by a 2.

<div class="row mt-5">
    <div class="col-sm mt-5 mt-md-0">
        {% include figure.liquid loading="eager" path="assets/img/2024-05-02-fft/8p6.png" class="img-fluid rounded z-depth-1" %}
    </div>
</div>

Ok, now the last time:  

<div class="row mt-5">
    <div class="col-sm mt-5 mt-md-0">
        {% include figure.liquid loading="eager" path="assets/img/2024-05-02-fft/8p7.png" class="img-fluid rounded z-depth-1" %}
    </div>
</div>

Not the $log_2N^th$ twiddle factor is $e^{-\frac{2\pi i 0* k}{1}} = 1$. So now the thing becomes to:  
  
<div class="row mt-5">
    <div class="col-sm mt-5 mt-md-0">
        {% include figure.liquid loading="eager" path="assets/img/2024-05-02-fft/8p8.png" class="img-fluid rounded z-depth-1" %}
    </div>
</div>

Rearrange them:  

<div class="row mt-5">
    <div class="col-sm mt-5 mt-md-0">
        {% include figure.liquid loading="eager" path="assets/img/2024-05-02-fft/8p9.png" class="img-fluid rounded z-depth-1" %}
    </div>
</div>

For those who have seen the butterfly diagram probably will shout out: *Oh that is the butterfly thing!* (That is what I did at the first time learning this topic). Do not forget the $k$ in the exponential! What does it mean? It means that for every $k$, the computer needs to go through every calculation one time. Beacuse the $k$ value varies and we need to compute everything again when meet a new $k$. Besides what we did just now is just doing rearrangement and this doesn't relieve any of the computational complexity.  So the time complexity till now is still $O(N^2)$.  **What the butterfly diagram tells us is that we can resuse the results at each stage(the separation of odd and even terms)**. But what we have acchieved cannot promise that.  

Now we comes to the most important part(I think because I spend days of time to figure out what's gonna be next)

## How to read a butterfly diagram

Next we will work through the whole thing with butterfly diagram as a reference. So let's read it first.  

* Each line(or arrow) is a multiplication by a factor(a constant)
* Each dot(end points of 2 lines) is an addition
* Each branch(start points of 2 branches) means the value after multiplication can go either way.  

Actually this graph clearly demostrates that the time complexity is $NlogN$. With the stage number of $log(N)$ and $N '+' and N '*'$ at each stage.  

<div class="row mt-3">
    <div class="col-sm mt-4 mt-md-0">
        {% include figure.liquid loading="eager" path="assets/img/2024-05-02-fft/butterfly.png" class="img-fluid rounded z-depth-1" %}
    </div>
</div>
<div class='caption'> A butterfly diagram.<d-cite key = 'C25_2'></d-cite></div>

## Connections with butterfly diagram:the elimination of k in twiddle factors

Let's re-look at the following equation:  
I delibrately write the equation in a form of even and odd terms.  
<div class="row mt-5">
    <div class="col-sm mt-5 mt-md-0">
        {% include figure.liquid loading="eager" path="assets/img/2024-05-02-fft/8p9.png" class="img-fluid rounded z-depth-1" %}
    </div>
</div>

For the $3^{rd}$ stage(the second left column), the twiddling factor is $W_{t3} = W_2 = e^{-\frac{2\pi i k}{2}}$  

$$W_{t3} = 1, k = even number$$
$$W_{t3} = -1, k = odd number$$

So no matter the $k$ in the third stage there can only be 2 options for a 2 point DFT.  We can reuse the data in the first stage!  

Now let's construct the butterfly diagram:  

If $k$ is even, we let the 0-4, 2-6, 1-5, 3-7 pair to combine and calculate a value and put it in the upper place. Just as the red line shows.  

<div class="row mt-5">
    <div class="col-sm-12 mt-5 mt-md-0">
        {% include figure.liquid loading="eager" path="assets/img/2024-05-02-fft/stage3even.png" class="img-fluid rounded z-depth-1" %}
    </div>
</div>

Vice versa, if $k$ is odd, just to the computation with a different twiddling factor and put it in the lower place. Just as the blue line shows.  

<div class="row mt-5">
    <div class="col-sm-12 mt-5 mt-md-0">
        {% include figure.liquid loading="eager" path="assets/img/2024-05-02-fft/stage3odd.png" class="img-fluid rounded z-depth-1" %}
    </div>
</div>

OK, now that's where we save the computation time. Originally, on the $3rd$ stage we need calculate $N * N/2 ('*' and '+')$. Now  we only need to calculate(N '*' and '+').  

And actually the same thing can be applied to the $2^{nd}$ stage and $1^{st}$ stage.  

We finished! You can derive the $2^{nd}$ stage and $1^{st}$ stage and construct the butterfly diagram by your self!  

## Broken matrixs

DFT matrix  
\[
    \begin{bmatrix}
        \hat f_0 \\
        \hat f_1 \\
        \vdots \\
        \hat f_{N-1} \\
    \end{bmatrix}
    = \frac{1}{N}
    \begin{bmatrix}
        1 & 1 & 1 & \dots & 1\\
        1 & W_N & W_N^2 & \dots & W_N^{N-1} \\
        \vdots & & & & \vdots \\
        1 & W_{N-1} & W_N^{2(N-1)} & \dots & W_N^{(N-1)^2}  \\
    \end{bmatrix}
    \begin{bmatrix}
        f_0 \\
        f_1 \\
        \vdots \\
        f_{N-1} \\
    \end{bmatrix}
\]

Code for 8-point equation 1-8  


* 1

\[
    \hat f[k]
    = \frac{1}{8}\sum_{n=0}^{7} e^{-\frac{2\pi ikn}{8}}
    =
    \begin{matrix}
        f[0]e^{-\frac{2\pi i 0* k}{8}} + f[2]e^{-\frac{2\pi i 2* k}{8}} + f[4]e^{-\frac{2\pi i 4* k}{8}} + f[6]e^{-\frac{2\pi i 6* k}{8}} \\
        +f[1]e^{-\frac{2\pi i 1* k}{8}} +f[3]e^{-\frac{2\pi i 3* k}{8}} +  f[5]e^{-\frac{2\pi i 5* k}{8}} + f[7]e^{-\frac{2\pi i 7* k}{8}} \\
    \end{matrix}
\]

* 2

\[
    \hat f[k]
    = \frac{1}{8}\sum_{n=0}^{7} e^{-\frac{2\pi ikn}{8}}
    =
    \begin{matrix}
        f[0]e^{-\frac{2\pi i 0* k}{8}} + f[2]e^{-\frac{2\pi i 2* k}{8}} + f[4]e^{-\frac{2\pi i 4* k}{8}} + f[6]e^{-\frac{2\pi i 6* k}{8}} \\
        +e^{-\frac{2\pi i k}{8}}(f[1]e^{-\frac{2\pi i 0* k}{8}} +f[3]e^{-\frac{2\pi i 2* k}{8}} +  f[5]e^{-\frac{2\pi i 4* k}{8}} + f[7]e^{-\frac{2\pi i 6* k}{8}}) \\
    \end{matrix}
\]

* 3

\[
    \hat f[k]
    = \frac{1}{8}\sum_{n=0}^{7} e^{-\frac{2\pi ikn}{8}}
    =
    \begin{matrix}
        f[0]e^{-\frac{2\pi i 0* k}{8}} + f[4]e^{-\frac{2\pi i 4* k}{8}} \\
        + f[2]e^{-\frac{2\pi i 2* k}{8}} + f[6]e^{-\frac{2\pi i 6* k}{8}} \\
        +e^{-\frac{2\pi i k}{8}}(f[1]e^{-\frac{2\pi i 0* k}{8}} +  f[5]e^{-\frac{2\pi i 4* k}{8}}) \\
        +e^{-\frac{2\pi i k}{8}}(f[3]e^{-\frac{2\pi i 2* k}{8}} +  f[7]e^{-\frac{2\pi i 6* k}{8}}) \\
    \end{matrix}
\]

* 4

\[
    \hat f[k]
    =
    \begin{matrix}
        f[0]e^{-\frac{2\pi i 0* k}{4}} + f[4]e^{-\frac{2\pi i 2* k}{4}} \\
        + f[2]e^{-\frac{2\pi i 1* k}{4}} + f[6]e^{-\frac{2\pi i 3* k}{4}} \\
        +e^{-\frac{2\pi i k}{8}}(f[1]e^{-\frac{2\pi i 0* k}{4}} +  f[5]e^{-\frac{2\pi i 2* k}{4}}) \\
        +e^{-\frac{2\pi i k}{8}}(f[3]e^{-\frac{2\pi i 1* k}{4}} +  f[7]e^{-\frac{2\pi i 3* k}{8}}) \\
    \end{matrix}
\]

* 5


\[
    \hat f[k]
    =
    \begin{matrix}
        f[0]e^{-\frac{2\pi i 0* k}{4}} + f[4]e^{-\frac{2\pi i 2* k}{4}} \\
        + e^{-\frac{2\pi i k}{4}}[f[2]e^{-\frac{2\pi i 0* k}{4}} + f[6]e^{-\frac{2\pi i 2* k}{4}}] \\
        +e^{-\frac{2\pi i k}{8}}\{f[1]e^{-\frac{2\pi i 0* k}{4}} +  f[5]e^{-\frac{2\pi i 2* k}{4}}\} \\
        +e^{-\frac{2\pi i k}{8}}\{e^{-\frac{2\pi i k}{4}}[f[3]e^{-\frac{2\pi i 0* k}{4}} +  f[7]e^{-\frac{2\pi i 2* k}{4}}]\} \\
    \end{matrix}
\]

* 6

\[
    \hat f[k]
    =
    \begin{matrix}
        f[0]e^{-\frac{2\pi i 0* k}{2}} + f[4]e^{-\frac{2\pi i 1* k}{2}} \\
        + e^{-\frac{2\pi i k}{4}}[f[2]e^{-\frac{2\pi i 0* k}{2}} + f[6]e^{-\frac{2\pi i 1* k}{2}}] \\
        +e^{-\frac{2\pi i k}{8}}\{f[1]e^{-\frac{2\pi i 0* k}{2}} +  f[5]e^{-\frac{2\pi i 1* k}{2}}\} \\
        +e^{-\frac{2\pi i k}{8}}\{e^{-\frac{2\pi i k}{4}}[f[3]e^{-\frac{2\pi i 0* k}{2}} +  f[7]e^{-\frac{2\pi i 1* k}{2}}]\} \\
    \end{matrix}
\]

* 7

\[
    \hat f[k]
    =
    \begin{matrix}
        f[0]e^{-\frac{2\pi i 0* k}{1}} \\
        +e^{-\frac{2\pi i 1* k}{2}} * f[4]e^{-\frac{2\pi i 0* k}{1}} \\
        + e^{-\frac{2\pi i k}{4}}[f[2]e^{-\frac{2\pi i 0* k}{1}}] \\
        + e^{-\frac{2\pi i k}{4}}[ e^{-\frac{2\pi i 1* k}{2}} * f[6]e^{-\frac{2\pi i 0* k}{1}}] \\
        +e^{-\frac{2\pi i k}{8}}\{f[1]e^{-\frac{2\pi i 0* k}{1}}\} \\
        +e^{-\frac{2\pi i k}{8}}\{e^{-\frac{2\pi i 1* k}{2}} * f[5]e^{-\frac{2\pi i 0* k}{1}}\} \\
        +e^{-\frac{2\pi i k}{8}}\{e^{-\frac{2\pi i k}{4}}[f[3]e^{-\frac{2\pi i 0* k}{1}}]\} \\
        +e^{-\frac{2\pi i k}{8}}\{e^{-\frac{2\pi i k}{4}}[e^{-\frac{2\pi i 1* k}{2}} f[7]e^{-\frac{2\pi i 0* k}{1}}]\} \\
    \end{matrix}
\]

* 8

\[
    \hat f[k]
    =
    \begin{matrix}
        f[0] \\
        +e^{-\frac{2\pi i 1* k}{2}} * f[4] \\
        + e^{-\frac{2\pi i k}{4}}[f[2]] \\
        + e^{-\frac{2\pi i k}{4}}[ e^{-\frac{2\pi i 1* k}{2}} * f[6]] \\
        +e^{-\frac{2\pi i k}{8}}\{f[1]\} \\
        +e^{-\frac{2\pi i k}{8}}\{e^{-\frac{2\pi i 1* k}{2}} * f[5]\} \\
        +e^{-\frac{2\pi i k}{8}}\{e^{-\frac{2\pi i k}{4}}[f[3]]\} \\
        +e^{-\frac{2\pi i k}{8}}\{e^{-\frac{2\pi i k}{4}}[e^{-\frac{2\pi i 1* k}{2}} f[7]]\} \\
    \end{matrix}
\]

* 9

\[
    \hat f[k]
    =
    \begin{matrix}
         & f[0] & & & \\
        + & f[4] & *e^{-\frac{2\pi i k}{2}}& & \\
        + & f[2]& & * e^{-\frac{2\pi i k}{4}} & \\
        + & f[6] &*e^{-\frac{2\pi i k}{2}}& *e^{-\frac{2\pi i k}{4}} & \\
        + & f[1] & & & *e^{-\frac{2\pi i k}{8}}\\
        + & f[5] & *e^{-\frac{2\pi i k}{2}}& & *e^{-\frac{2\pi i k}{8}}\\
        + & f[3]& & * e^{-\frac{2\pi i k}{4}} & *e^{-\frac{2\pi i k}{8}}\\
        + & f[7] &*e^{-\frac{2\pi i k}{2}}& *e^{-\frac{2\pi i k}{4}} & *e^{-\frac{2\pi i k}{8}}\\
    \end{matrix}
\]